impl/src/verifier/fstar_files/NSMain__main_main.fst
@@ -28,8 +28,8 @@ let nSMain__emptyArgs  =
   let __return = ___ir_ret__ in
   __return
 
-val fn___home_jose_Documents_GithubProjects_BosqueLanguage_impl_src_test_apps_max_main_bsq_235_0 : (x:bosqueTerm{subtypeOf BIntType (getType x)}) -> (x:bosqueTerm{subtypeOf BIntType (getType x)}) -> (x:bosqueTerm{subtypeOf BIntType (getType x)}) -> Tot (x:bosqueTerm{subtypeOf BIntType (getType x)})
-let fn___home_jose_Documents_GithubProjects_BosqueLanguage_impl_src_test_apps_max_main_bsq_235_0 x y __c_access_example = 
+val fn___home_jose_Documents_GithubProjects_BosqueLanguage_impl_src_test_apps_max_main_bsq_235__5605 : (x:bosqueTerm{subtypeOf BIntType (getType x)}) -> (x:bosqueTerm{subtypeOf BIntType (getType x)}) -> (x:bosqueTerm{subtypeOf BIntType (getType x)}) -> Tot (x:bosqueTerm{subtypeOf BIntType (getType x)})
+let fn___home_jose_Documents_GithubProjects_BosqueLanguage_impl_src_test_apps_max_main_bsq_235__5605 x y __c_access_example = 
   let _ = assert_norm(subtypeOf BIntType (getType __c_access_example)) in
   let _ = assert_norm(subtypeOf BIntType (getType y)) in
   let __tmp_2 = (op_add y __c_access_example) in
@@ -48,7 +48,7 @@ let nSMain__foo__home_jose_Documents_GithubProjects_BosqueLanguage_impl_src_test
   let _ = assert_norm(subtypeOf BIntType (getType __c_access_example)) in
   let _ = assert_norm(subtypeOf BIntType (getType __tmp_4)) in
   let _ = assert_norm(subtypeOf BIntType (getType __tmp_3)) in
-  let __tmp_0 = (fn___home_jose_Documents_GithubProjects_BosqueLanguage_impl_src_test_apps_max_main_bsq_235_0 __tmp_3 __tmp_4 __c_access_example) in
+  let __tmp_0 = (fn___home_jose_Documents_GithubProjects_BosqueLanguage_impl_src_test_apps_max_main_bsq_235__5605 __tmp_3 __tmp_4 __c_access_example) in
   let ___ir_ret__ = __tmp_0 in
   let __return = ___ir_ret__ in
   __return
@@ -56,13 +56,13 @@ let nSMain__foo__home_jose_Documents_GithubProjects_BosqueLanguage_impl_src_test
 val nSMain__main : (x:bosqueTerm{subtypeOf BIntType (getType x)})
 let nSMain__main  = 
   let __tmp_4 = nSMain__Baz2_zexample_default in
-  let __tmp_0_arg_3 = (BInt 12) in
-  let __tmp_0_arg_2 = __tmp_4 in
-  let __tmp_0_arg_1 = (BBool true) in
-  let __tmp_0_arg_0 = (BInt 34) in
+  let __tmp_0_arg_3 = __tmp_4 in
+  let __tmp_0_arg_2 = (BBool true) in
+  let __tmp_0_arg_1 = (BInt 34) in
+  let __tmp_0_arg_0 = (BInt 12) in
   let _ = assert_norm(subtypeOf BIntType (getType __tmp_0_arg_3)) in
-  let _ = assert_norm(subtypeOf BIntType (getType __tmp_0_arg_2)) in
-  let _ = assert_norm(subtypeOf BBoolType (getType __tmp_0_arg_1)) in
+  let _ = assert_norm(subtypeOf BBoolType (getType __tmp_0_arg_2)) in
+  let _ = assert_norm(subtypeOf BIntType (getType __tmp_0_arg_1)) in
   let _ = assert_norm(subtypeOf BIntType (getType __tmp_0_arg_0)) in
   let __tmp_0 = (BnSMain__Baz2 __tmp_0_arg_0 __tmp_0_arg_1 __tmp_0_arg_2 __tmp_0_arg_3) in
   let e = __tmp_0 in
